DDH ≤ ot_sim

theories/prob_eff_lang/probblaze/examples/ot/OT_Scorrupt_mut.v
@@ -106,11 +106,11 @@ Section handlee_verification.
   (* Theories for the client *)
   (*------------------------------------------------------------*)
   
-  Program Definition SenderTheory : iThy Σ :=
-    λ e1 e2, (λne Q, ∃ m0 m1 : vgG,
-                ⌜ e1 = do: Sender (m0, m1)%V ⌝%E ∗
-                ⌜ e2 = do: Sender (m0, m1)%V ⌝%E ∗
-                (Q #()%V #()%V)
+  Program Definition ReceiverTheory : iThy Σ :=
+    λ e1 e2, (λne Q, ∃ b : bool,
+                ⌜ e1 = do: Receiver #b ⌝%E ∗
+                ⌜ e2 = do: Receiver #b ⌝%E ∗
+                ((Q NONEV NONEV) ∗ (∀ m : val, Q (SOMEV m) (SOMEV m)) ∗ (Q #()%V #()%V) )  
              )%I.
   Next Obligation. solve_proper. Qed.
 
@@ -149,8 +149,8 @@ Section handlee_verification.
     λ e1 e2, (λne Q,
                 ⌜ e1 = do: channel (RecvV bob) ⌝%E ∗
                 ⌜ e2 = do: channel (RecvV bob) ⌝%E ∗
-                (* Added a later, since RHS doesn't take a step *)
-                ▷ (Q NONEV NONEV ∗ (∀ m, own γauth (to_dfrac_agree DfracDiscarded m) -∗ Q (SOMEV m) (SOMEV m)))
+                (* Added a later, since RHS doesn't take a step. Conjunction is because a one-shot cont is resumed in either branch *)
+                ▷ (Q NONEV NONEV ∧ (∀ c0 d0 c1 d1 : vgG, own γauth (to_dfrac_agree DfracDiscarded ((c0, d0), (c1, d1))%V) -∗ Q (SOMEV ((c0,d0),(c1,d1))) (SOMEV ((c0,d0),(c1,d1)))))
              )%I.
   Next Obligation. solve_proper. Qed.
 
@@ -169,7 +169,7 @@ Section handlee_verification.
 
   Definition LblAdv γcrs γtokb γfracb γauthb btokN := [([CRS],[CRS], @CRSThy γcrs);([channel], [channel],
                                                                            (iThySum (SendBobImpl γtokb γfracb γauthb btokN) (RecvBobImpl γauthb)));
-                                                                         ([Sender],[Sender;Receiver;Leak],SenderTheory)].
+                                                                         ([Receiver],[Sender;Receiver;Leak],ReceiverTheory)].
   Definition LblAuthChannel γtoka atokN γtokb btokN γfraca γfracb γautha γauthb := [([channel],[channel], (iThySum (iThySum (SendAliceImpl γtoka γfraca γautha atokN) (RecvBobImpl γauthb))
                                                                         (iThySum (SendBobImpl γtokb γfracb γauthb btokN) (RecvAliceImpl γautha))))].
 
@@ -253,22 +253,370 @@ Admitted.
        CRS ≠ channel → *)
     let AuthChannel := LblAuthChannel γtoka atokN γtokb btokN γfraca γfracb γautha γauthb in
     let Adv := LblAdv γcrs γtokb γfracb γauthb btokN in
-    token γtokb -∗
+    token γtoka -∗
     own γcrs (to_dfrac_agree (DfracOwn 1) #()%V) -∗
-    own γauthb (to_dfrac_agree (DfracOwn 1) #()%V) -∗
+    own γautha (to_dfrac_agree (DfracOwn 1) #()%V) -∗
     BREL f1 #()%V ≤ f2 #()%V <| (Adv ++ L)|> {{ (λ v1 v2, ⌜v1 = #()%V ∧ v2 = #()%V⌝) }} -∗
     
     ↯ (1 / n) -∗
 
     BREL F_CRS CRS (OT_Real_Sender_corrupt CRS Receiver channel  f1) 
       ≤ (reduction CRS DH_rand) (OT_Real_Sender_corrupt CRS Receiver channel f2)
-      <| (([CRS],[CRS], iThyBot) :: ([Sender],[Sender; Receiver; Leak],iThyBot) :: AuthChannel ++ L) |>  {{ (λ v1 v2, ⌜ v1 = v2 ⌝) }}. 
+      <| (([CRS],[CRS], iThyBot) :: ([Receiver],[Sender; Receiver; Leak],iThyBot) :: AuthChannel ++ L) |>  {{ (λ v1 v2, ⌜ v1 = v2 ⌝) }}. 
   Proof. 
     iIntros (????) "Htoken Hcrs Hauth Hff Herr".
     unfold OT_Real_Sender_corrupt. brel_pures.
     iApply (fcrs_dh_ideal with "[$][$Hcrs]").
     (* Prove that OT_Real_Sender_corrupt is related to it self *)
+    (* Also consider changing the types, if it is necessary *)
   Admitted.
+
+
+  
+  Lemma DH_OT_sim  (f1 f2 : val) m0 m1 γcrs γtoka γtokb γfraca γfracb γautha γauthb L :
+    let AuthChannel := LblAuthChannel γtoka atokN γtokb btokN γfraca γfracb γautha γauthb in
+    let Adv := LblAdv γcrs γtokb γfracb γauthb btokN in
+    token γtoka -∗
+    own γcrs (to_dfrac_agree (DfracOwn 1) #()%V) -∗
+    own γautha (to_dfrac_agree (DfracOwn 1) #()%V) -∗
+    m0 ↦ₛ NONEV -∗
+    m1 ↦ₛ NONEV -∗
+    BREL f1 #()%V ≤ f2 #()%V <| (Adv ++ L)|> {{ (λ v1 v2, ⌜v1 = #()%V ∧ v2 = #()%V⌝) }} -∗
+    BREL (reduction CRS DH_real) (OT_Real_Sender_corrupt CRS Receiver channel f1) 
+      ≤ (OT_SIM_FOT channel CRS Sender Receiver Leak m0 m1) f2 <| to_iThyIfMono OS (([CRS],[CRS], iThyBot) :: ([Receiver],[Sender; Receiver; Leak],iThyBot) :: AuthChannel ++ L) |>  {{ (λ v1 v2, ⌜ v1 = v2 ⌝) }}.
+  Proof.  
+    iIntros (??) "Htok Hcrs Hauth Hlm0 Hlm1 Hff".
+    rewrite /reduction /OT_Real_Sender_corrupt /OT_SIM_FOT /DH_real /OT_SIM /F_OT //=.
+    brel_pures.
+    iApply brel_couple_rand_rand; first done. iIntros (t Ht). brel_pures'.
+    iApply brel_couple_rand_rand; first done. iIntros (y Hy). brel_pures'. (* should be non-zero *)
+    iApply brel_couple_rand_rand; first done. iIntros (x Hx). brel_pures'. 
+    rewrite -Nat2Z.inj_mul. 
+    rewrite /OT_SIM_Sender_corrupt_logic /mutual_handlers_composition.mut_handler_constructor.
+    brel_pures'.
+    rewrite expgnA.
+
+    iApply fupd_brel.
+    iDestruct (auth_upd  (vgval (g ^+ t ^+ y ^+ x), vgval (g ^+ t ^+ x), vgval (g ^+ t ^+ y), vgval (g ^+ t))%V with "Hcrs") as ">Hcrs".
+    iDestruct (auth_persist with "Hcrs") as ">Hcrs". 
+    iDestruct "Hcrs" as "#Hcrs". 
+    iModIntro.
+
+    iApply fupd_brel.
+    iMod (inv_alloc atokN _ (token γtoka ∗ own γautha (to_dfrac_agree (DfracOwn 1) #()%V) ∨ own γfraca DfracDiscarded)%I with "[Htok Hauth]") as "#Hinvt".
+    { iNext; iLeft;iFrame. }
+    iModIntro.
+    
+    (* CRS *)
+    iApply (brel_exhaustion _ _ [_] [_] (iThyMono (iThySum CRSThy CRSThyL)) with "[Hff Hlm0 Hlm1]"); [done|done| |].
+
+    (* CRS handler *)
+    2 : { iLöb as "IH".
+          iSplit; [iIntros (v1 v2) "!# H"; by brel_pures'|].
+          iIntros (???????) "!# (%&[(->&->&HQ)| (->&HQ)]&HQQ) #Hkont".
+          - iApply brel_handle_os_l; [apply neutral_ectx; set_solver|].
+            iIntros (rl) "!> Hrl".
+            iApply brel_handle_os_r; [apply neutral_ectx; set_solver|].
+            iIntros (rr) "Hrr".
+            brel_pures'.
+            iApply (brel_cont_l with "[$]"). iModIntro.
+            iApply (brel_cont_r with "[$]").
+            iDestruct ("HQ" with "Hcrs") as "HQ'".
+            iDestruct ("HQQ" with "HQ'") as "HQ".
+            iDestruct ("Hkont" with "HQ") as "H".
+            iApply (brel_exhaustion _ _ [_] [_] (iThyMono (iThySum CRSThy CRSThyL)) with "[H]"); done.
+          - iApply brel_handle_os_l; [apply neutral_ectx; set_solver|].
+            iIntros (rl) "!> Hrl". brel_pures'.
+            iApply (brel_cont_l with "[$]"). iModIntro.
+            iDestruct ("HQ" with "Hcrs") as "HQ'".
+            iDestruct ("HQQ" with "HQ'") as "HQ".
+            iDestruct ("Hkont" with "HQ") as "H".
+            iApply (brel_exhaustion _ _ [_] [_] (iThyMono (iThySum CRSThy CRSThyL)) with "[H]"); done. }
+
+     (* Manipulation of theories *)
+    iApply brel_introduction_mono. { iApply to_iThy_le_intro'. eapply submseteq_swap. }
+    iDestruct (brel_introduction_mono _ with "[][$Hff]") as "Hff".
+    { iApply to_iThy_le_trans.
+      (* add CRSThyL to the row of ff just to match the row of the context in the rest of the proof. It's fine since we've already factored out the CRS handler *)
+      - iSplit.
+        { iApply iThy_le_trans; first iApply (iThy_le_to_iThy_sum [CRS] [CRS]).
+          iApply iThy_le_trans; last iApply (iThy_le_sum_to_iThy [CRS] [CRS] ((iThySum CRSThy CRSThyL))).
+          iApply iThy_le_sum_l. iIntros (???) "!# (%&%&%&%&%&?&?&?&?&H&?)". iExists e1',e2',k1,k2,_. iFrame. }
+        iSplit; iModIntro; [iIntros "#Hvalid"; iApply valid_to_iThy_bot; by (iDestruct (valid_to_iThy_bot with "Hvalid") as "?")| (iIntros (Hdistinct); iPureIntro)]; simpl.
+        apply distinct_to_iThy_bot. by apply distinct_to_iThy_bot in Hdistinct. 
+      - iApply to_iThy_le_intro'. eapply submseteq_trans; last first.
+           +  eapply submseteq_skip. eapply submseteq_swap.
+           +  eapply submseteq_swap. }
+
+     iDestruct (brel_introduction_mono _ (AuthChannel ++ [([Receiver],[Sender;Receiver;Leak], ReceiverTheory); ([CRS], [CRS], iThySum CRSThy CRSThyL)] ++ L) with "[][$Hff]") as "Hff". 
+    {  iSplit.
+       + iApply iThy_le_trans; [iApply iThy_le_to_iThy_sum|].
+         iApply iThy_le_trans; [|iApply iThy_le_sum_to_iThy].
+         iApply iThy_le_sum_l. iIntros (???) "!#  (%&%&%&%&%&?&?&H)". iExists _,_,_,_,_. iFrame.
+         iDestruct "H" as "(?&?&HX&#HSQ)". iFrame. iSplitL "HX"; [|iApply "HSQ"].
+         iDestruct "HX" as "[HX | HX]"; [iRight;iLeft;done|iLeft;iRight;done].
+       + iSplit; iModIntro; [iApply valid_submseteq'|iIntros (Hdistinct'); iPureIntro; eapply distinct_submseteq'; last done]; simpl;
+           try rewrite !labels_l_cons; try rewrite !labels_r_cons; set_solver.
+    }
+    iDestruct (brel_introduction_mono _ with "[][$Hff]") as "Hff".
+    { iApply to_iThy_le_intro'. eapply submseteq_trans; first eapply submseteq_swap.
+      eapply submseteq_skip. eapply submseteq_swap. }
+    
+    iApply (brel_exhaustion' OS (f1 #()%V) (f2 #()%V) with "[$Hff]"); [done|set_solver|].
+    iSplit; [iIntros (v1 v2) "(->&->)"; by brel_pures|].
+    iIntros (k1' k2' e1' e2' Q Hk1' Hk2') "(%&->&->&(HQNone & HQSome & _)) Hkont".
+    iApply brel_handle_os_l; [apply neutral_ectx;set_solver|].
+    iIntros (cl) "!> Hcl". brel_pures'.
+    iApply (brel_handle_os_r [_] ([HandleCtx _ _ _ _ _] ++ k2')). 
+    { simpl. admit. }                    (* known from brel_learn *)
+    iIntros (cr) "Hcr".
+    brel_pures'.
+    iApply (brel_handle_os_r [] [AppRCtx _]); [set_solver|simpl].
+    iIntros (cleak) "Hleak".
+    brel_pures'.
+    iApply (brel_introduction' [CRS]). { repeat constructor. }
+    iExists _, _, [AppRCtx _], [], _.  iSplit; [done|].
+    iSplit; [iPureIntro; apply AppRCtx_NeutralEctx; apply NeutralEctx_nil|].
+    iSplit; [done|]. iSplit; [iPureIntro; apply NeutralEctx_nil|].
+    iSplit; last (iModIntro; iIntros (??) "H"; done).
+    iExists _. iSplitL; last (iIntros (??) "!> H"; iApply "H").
+    iRight. iSplit; [done|]. iIntros (?) "Hcrs'".
+    iDestruct (auth_agree with "[$][$]") as "->". iClear "Hcrs'".
+    brel_pures'.
+
+    (* Should be refactored into one branch *)
+    destruct b.
+    - epose proof brel_couple_rand_rand as h'.
+      unshelve iApply (h' _ _ (@f_ring n'' (zmodp.inZp y)) (f_bij_ring (zmodp.inZp y))); try done.
+      { admit. }
+      { intros n Hlt. apply Rcomplements.SSR_leq. unshelve eapply f_lt_ring; first done.
+        by apply Rcomplements.SSR_leq. }
+      iIntros (α Hα).
+      brel_pures'. rewrite -Nat2Z.inj_mul. brel_pures'.
+      rewrite -expgM. rewrite ssrnat.multE. rewrite (ssrnat.mulnC _ y).
+      (* rewrite -(@expg_mod _ n (ssrnat.muln y (f_ring (zmodp.inZp y) α))).
+         2 : admit. *)
+      assert (ssrnat.muln y (f_ring (zmodp.inZp y) α) = α) as -> by admit.
+
+      iApply (brel_introduction' [channel]); [repeat constructor|].
+      iExists _,_,[AppRCtx _],[HandleCtx _ _ _ _ _ ;HandleCtx _ _ _ _ _;HandleCtx _ _ _ _ _;AppRCtx _],_.
+      iSplit; [by iPureIntro|]. 
+      iSplit; [iPureIntro; apply NeutralEctx_ectx_labels_singleton; set_solver| ].
+      iSplit; [by iPureIntro|].
+      iSplit; [iPureIntro; apply NeutralEctx_ectx_labels_singleton; admit| ]. (* from brel_learn *)
+      iSplitL; [|iIntros (??) "!# H"; iApply "H"].
+      iExists _. iSplitL; last (iIntros (??) "!> H"; iApply "H").
+      iLeft. iLeft. 
+      iExists _,_.
+      iSplitR.
+      { iMod (inv_acc with "Hinvt") as "([>(Htok & Hagree) | >#Hfrac] & Hclose)"; try done.
+        - iModIntro. iLeft. iIntros "#Hfrac".
+          iMod (auth_upd (vgval (g ^+ t ^+ α), vgval (g ^+ t ^+ x ^+ α))%V
+                 with "Hagree") as "Hagree".
+          iMod (auth_persist with "Hagree") as "#Hagree".
+          iFrame. iMod ("Hclose" with "[$]") as "_". iFrame "#".
+          by iModIntro.
+        - iRight. iFrame "#".
+          iModIntro. iApply "Hclose". iNext.
+          by iRight. }
+      iSplit; [iSplit;done|].
+      iModIntro. simpl.
+      brel_pures'.
+      
+      iApply (brel_introduction' [channel]); [repeat constructor|].
+      iExists _,_,[AppRCtx _],[HandleCtx _ _ _ _ _ ;HandleCtx _ _ _ _ _;HandleCtx _ _ _ _ _;AppRCtx _],_.
+      iSplit; [by iPureIntro|]. 
+      iSplit; [iPureIntro; apply NeutralEctx_ectx_labels_singleton; set_solver| ].
+      iSplit; [by iPureIntro|].
+      iSplit; [iPureIntro; apply NeutralEctx_ectx_labels_singleton; admit| ]. (* from brel_learn *)
+      iSplitL; [|iIntros (??) "!# H"; iApply "H"].
+      iExists _. iSplitL; last (iIntros (??) "!> H"; iApply "H").
+      iLeft. iRight.
+      do 2 (iSplit; [done|]).
+      iModIntro.
+      iSplit.
+
+      (* Protocol done loop *)
+      { brel_pures'.
+        iDestruct ("Hkont" with "HQNone") as "Hfill".
+        iApply (brel_cont_l with "[$]"). iModIntro.
+        iApply (brel_cont_r with "[$]").
+        brel_pures'.
+        iApply (brel_load_r with "[$Hlm0]"). iIntros "Hlm0". brel_pures.
+        iApply (brel_cont_r with "[$]").
+        iClear "Hlm0 Hlm1 HQSome".
+        iApply (brel_exhaustion' OS (fill _ (InjLV #()%V)) (fill _ (InjLV #()%V)) _ _ _ _
+                  (([CRS],[CRS], _) :: AuthChannel ++ L) with "Hfill"); [set_solver|set_solver|].
+        iLöb as "IH". 
+        iSplit; [iIntros (v1 v2) "(->&->)"; by brel_pures|].
+        iIntros (k1'' k2'' ?????) "(%&->&->&(HQNone & HQSome & Hdone)) Hkont".
+        iApply brel_handle_os_l; [apply neutral_ectx;set_solver| ].
+        iIntros (rl) "!> Hrl". 
+        iApply (brel_handle_os_r _ ([HandleCtx _ _ _ _ _] ++ k2'')). { admit. } (* from brel_learn *)
+        iIntros (rr) "Hrr". 
+        brel_pures'.
+        iApply (brel_cont_l with "[$]"). iModIntro.
+        iApply (brel_cont_r with "[$]").
+        iDestruct ("Hkont" with "Hdone") as "Hfill".
+          iApply (brel_exhaustion' OS (fill _  #()%V) (fill _ #()%V) _ _ _ _
+                  (([CRS],[CRS], _) :: AuthChannel ++ L) with "Hfill"); [set_solver|set_solver|].
+        by iApply "IH". }
+
+      iIntros (c0 d0 c1 d1) "#Hauth". 
+      brel_pures_r. 
+      repeat (first [brel_exp_l|brel_mult_l|brel_inv_l]).
+      (* do 5 (first [brel_exp_r|brel_mult_r|brel_inv_r]). *)
+      brel_pures_l. repeat (first [brel_exp_l|brel_mult_l|brel_inv_l]).
+      brel_pures'.
+      iApply (brel_handle_os_r [_;_] [AppRCtx _]); [set_solver|].
+      iIntros (rS) "HrS". brel_pures'.
+      unfold store_if_none.
+      iApply (brel_load_r with "Hlm0"). iIntros "Hlm0".
+      iApply (brel_store_r with "Hlm0"). iIntros "Hlm0".
+      brel_pures'.
+      iApply (brel_load_r with "Hlm1"). iIntros "Hlm1".
+      iApply (brel_store_r with "Hlm1"). iIntros "Hlm1".
+      brel_pures'.
+      iApply (brel_handle_os_r [] [HandleCtx _ _ _ _ _; AppRCtx _]); [admit|]. (* brel_learn *)
+      iIntros (rL) "HrL". brel_pures'.
+      iApply (brel_cont_r with "[$]").
+      brel_pures'.
+      iApply (brel_cont_r with "[$]"). brel_pures'.
+      iApply (brel_cont_r with "[$]"). brel_pures'.
+      iApply (brel_load_r with "[$Hlm0]"). iIntros "Hlm0". 
+      iApply (brel_cont_r with "[$]").
+      iApply (brel_cont_l with "[$]"). iModIntro.
+      iDestruct ("Hkont" with "HQSome") as "Hkont".
+      
+      iApply (brel_exhaustion' OS (fill k1' _) (fill k2' _) with "Hkont"); [done|set_solver|].
+      iClear "HQNone Hlm1 Hlm0".
+      iLöb as "IH".
+      iSplit; [iIntros (v1 v2) "(->&->)"; by brel_pures|].
+      iIntros (k1'' k2'' ?????) "(%&->&->&(HQNone & HQSome & Hdone)) Hkont".
+      iApply brel_handle_os_l; [apply neutral_ectx;set_solver| ].
+      iIntros (rl) "!> Hrl". 
+      iApply (brel_handle_os_r _ ([HandleCtx _ _ _ _ _] ++ k2'')). { admit. } (* from brel_learn *)
+      iIntros (rr) "Hrr". 
+      brel_pures'.
+      iApply (brel_cont_l with "[$]"). iModIntro.
+      iApply (brel_cont_r with "[$]").
+      iDestruct ("Hkont" with "Hdone") as "Hfill".
+      iApply (brel_exhaustion' OS (fill _  #()%V) (fill _ #()%V) _ _ _ _
+                (([CRS],[CRS], _) :: AuthChannel ++ L) with "Hfill"); [set_solver|set_solver|].
+      by iApply "IH".
+
+    - iApply brel_couple_rand_rand; first done. iIntros (α Hα).
+      brel_pures'. rewrite -Nat2Z.inj_mul. brel_pures'.
+             
+      iApply (brel_introduction' [channel]); [repeat constructor|].
+      iExists _,_,[AppRCtx _],[HandleCtx _ _ _ _ _ ;HandleCtx _ _ _ _ _;HandleCtx _ _ _ _ _;AppRCtx _],_.
+      iSplit; [by iPureIntro|]. 
+      iSplit; [iPureIntro; apply NeutralEctx_ectx_labels_singleton; set_solver| ].
+      iSplit; [by iPureIntro|].
+      iSplit; [iPureIntro; apply NeutralEctx_ectx_labels_singleton; admit| ]. (* from brel_learn *)
+      iSplitL; [|iIntros (??) "!# H"; iApply "H"].
+      iExists _. iSplitL; last (iIntros (??) "!> H"; iApply "H").
+      iLeft. iLeft. 
+      iExists _,_.
+      iSplitR.
+      { iMod (inv_acc with "Hinvt") as "([>(Htok & Hagree) | >#Hfrac] & Hclose)"; try done.
+        - iModIntro. iLeft. iIntros "#Hfrac".
+          iMod (auth_upd (vgval (g ^+ t ^+ y ^+ α), vgval (g ^+ t ^+ y ^+ x ^+ α))%V
+                 with "Hagree") as "Hagree".
+          iMod (auth_persist with "Hagree") as "#Hagree".
+          iFrame. iMod ("Hclose" with "[$]") as "_". iFrame "#".
+          by iModIntro.
+        - iRight. iFrame "#".
+          iModIntro. iApply "Hclose". iNext.
+          by iRight. }
+      rewrite !expgnA. rewrite expgnAC.
+      rewrite (expgnAC _ α y). rewrite (expgnAC _ x y).
+      iSplit; [iSplit;done|].  
+      iModIntro. simpl.
+      brel_pures'.
+      
+      iApply (brel_introduction' [channel]); [repeat constructor|].
+      iExists _,_,[AppRCtx _],[HandleCtx _ _ _ _ _ ;HandleCtx _ _ _ _ _;HandleCtx _ _ _ _ _;AppRCtx _],_.
+      iSplit; [by iPureIntro|]. 
+      iSplit; [iPureIntro; apply NeutralEctx_ectx_labels_singleton; set_solver| ].
+      iSplit; [by iPureIntro|].
+      iSplit; [iPureIntro; apply NeutralEctx_ectx_labels_singleton; admit| ]. (* from brel_learn *)
+      iSplitL; [|iIntros (??) "!# H"; iApply "H"].
+      iExists _. iSplitL; last (iIntros (??) "!> H"; iApply "H").
+      iLeft. iRight. simpl.
+      do 2 (iSplit; [done|]).
+      iModIntro.
+      iSplit.
+
+      (* Protocol done loop *)
+      { brel_pures'.
+        iDestruct ("Hkont" with "HQNone") as "Hfill".
+        iApply (brel_cont_l with "[$]"). iModIntro.
+        iApply (brel_cont_r with "[$]").
+        brel_pures'.
+        iApply (brel_load_r with "[$Hlm1]"). iIntros "Hlm1". brel_pures.
+        iApply (brel_cont_r with "[$]").
+        iClear "Hlm0 Hlm1 HQSome".
+        iApply (brel_exhaustion' OS (fill _ (InjLV #()%V)) (fill _ (InjLV #()%V)) _ _ _ _
+                  (([CRS],[CRS], _) :: AuthChannel ++ L) with "Hfill"); [set_solver|set_solver|].
+        iLöb as "IH". 
+        iSplit; [iIntros (v1 v2) "(->&->)"; by brel_pures|].
+        iIntros (k1'' k2'' ?????) "(%&->&->&(HQNone & HQSome & Hdone)) Hkont".
+        iApply brel_handle_os_l; [apply neutral_ectx;set_solver| ].
+        iIntros (rl) "!> Hrl". 
+        iApply (brel_handle_os_r _ ([HandleCtx _ _ _ _ _] ++ k2'')). { admit. } (* from brel_learn *)
+        iIntros (rr) "Hrr". 
+        brel_pures'.
+        iApply (brel_cont_l with "[$]"). iModIntro.
+        iApply (brel_cont_r with "[$]").
+        iDestruct ("Hkont" with "Hdone") as "Hfill".
+          iApply (brel_exhaustion' OS (fill _  #()%V) (fill _ #()%V) _ _ _ _
+                  (([CRS],[CRS], _) :: AuthChannel ++ L) with "Hfill"); [set_solver|set_solver|].
+        by iApply "IH". }
+
+      iIntros (c0 d0 c1 d1) "#Hauth". 
+      brel_pures.
+      repeat (first [brel_exp_l|brel_mult_l|brel_inv_l]).
+      do 5 (first [brel_exp_r|brel_mult_r|brel_inv_r]).
+      brel_pures'.
+      iApply (brel_handle_os_r [_;_] [AppRCtx _]); [set_solver|].
+      iIntros (rS) "HrS". brel_pures'.
+      unfold store_if_none.
+      iApply (brel_load_r with "Hlm0"). iIntros "Hlm0".
+      iApply (brel_store_r with "Hlm0"). iIntros "Hlm0".
+      brel_pures'.
+      iApply (brel_load_r with "Hlm1"). iIntros "Hlm1".
+      iApply (brel_store_r with "Hlm1"). iIntros "Hlm1".
+      brel_pures'.
+      iApply (brel_handle_os_r [] [HandleCtx _ _ _ _ _; AppRCtx _]); [admit|]. (* brel_learn *)
+      iIntros (rL) "HrL". brel_pures'.
+      iApply (brel_cont_r with "[$]").
+      brel_pures'.
+      iApply (brel_cont_r with "[$]"). brel_pures'.
+      iApply (brel_cont_r with "[$]"). brel_pures'.
+      iApply (brel_load_r with "[$Hlm1]"). iIntros "Hlm1". 
+      iApply (brel_cont_r with "[$]").
+      iApply (brel_cont_l with "[$]"). iModIntro.
+      iDestruct ("Hkont" with "HQSome") as "Hkont".
+
+      iApply (brel_exhaustion' OS (fill k1' _) (fill k2' _) with "Hkont"); [done|set_solver|].
+      iClear "HQNone Hlm1 Hlm0".
+      iLöb as "IH".
+      iSplit; [iIntros (v1 v2) "(->&->)"; by brel_pures|].
+      iIntros (k1'' k2'' ?????) "(%&->&->&(HQNone & HQSome & Hdone)) Hkont".
+      iApply brel_handle_os_l; [apply neutral_ectx;set_solver| ].
+      iIntros (rl) "!> Hrl". 
+      iApply (brel_handle_os_r _ ([HandleCtx _ _ _ _ _] ++ k2'')). { admit. } (* from brel_learn *)
+      iIntros (rr) "Hrr". 
+      brel_pures'.
+      iApply (brel_cont_l with "[$]"). iModIntro.
+      iApply (brel_cont_r with "[$]").
+      iDestruct ("Hkont" with "Hdone") as "Hfill".
+      iApply (brel_exhaustion' OS (fill _  #()%V) (fill _ #()%V) _ _ _ _
+                (([CRS],[CRS], _) :: AuthChannel ++ L) with "Hfill"); [set_solver|set_solver|].
+      by iApply "IH". 
+Admitted. 
+
 
 End handlee_verification.    
     
